theories/ordinals/Ackermann/checkPrf.v
@@ -63,7 +63,6 @@ Let apply := apply L.
 Let Formula := Formula L.
 Let equal := equal L.
 Let atomic := atomic L.
-Let impH := impH L.
 Let notH := notH L.
 Let forallH := forallH L.
 Let wellFormedTerm := wellFormedTerm codeArityF.
@@ -1197,7 +1196,7 @@ Definition checkPrfEQ2 (p recs : nat) :=
   charFunction 2 Nat.eqb (cdr (cdr p)) 0 *
     charFunction 2 Nat.eqb
       (codeFormula L codeF codeR
-         (fol.impH L (fol.equal L (fol.var L 0) (fol.var L 1))
+         (fol.impH (fol.equal L (fol.var L 0) (fol.var L 1))
             (fol.equal L (fol.var L 1) (fol.var L 0)))) 
       (car p).
 
@@ -1210,8 +1209,8 @@ Definition checkPrfEQ3 (p recs : nat) :=
   charFunction 2 Nat.eqb (cdr (cdr p)) 0 *
     charFunction 2 Nat.eqb
       (codeFormula L codeF codeR
-         (fol.impH L (fol.equal L (fol.var L 0) (fol.var L 1))
-            (fol.impH L (fol.equal L (fol.var L 1) (fol.var L 2))
+         (fol.impH (fol.equal L (fol.var L 0) (fol.var L 1))
+            (fol.impH (fol.equal L (fol.var L 1) (fol.var L 2))
                (fol.equal L (fol.var L 0) (fol.var L 2))))) 
       (car p).
 
@@ -1963,7 +1962,7 @@ Proof.
                 (cPair 1
                    (cPair (codeFormula L codeF codeR A0)
                       (codeFormula L codeF codeR B)))
-                (codePrf L codeF codeR Axm1 (fol.impH L A0 B) p1))
+                (codePrf L codeF codeR Axm1 (fol.impH  A0 B) p1))
              (cPair (codeFormula L codeF codeR A0) 
                 (codePrf L codeF codeR Axm2 A0 p0)))
       in *.
@@ -1980,7 +1979,7 @@ Proof.
           (cPair 1
              (cPair (codeFormula L codeF codeR A0) 
                 (codeFormula L codeF codeR B)))
-          with (codeFormula L codeF codeR (fol.impH L A0 B)); 
+          with (codeFormula L codeF codeR (impH A0 B)); 
           [ idtac | reflexivity ].
         rewrite Hrecp1.
         rewrite
@@ -2131,7 +2130,7 @@ Repeat First [Rewrite cPairProjections1|Rewrite cPairProjections2].
       unfold checkPrfEQ2 in |- *.
       replace
         (codeFormula L codeF codeR
-           (fol.impH L (fol.equal L (fol.var L 0) (fol.var L 1))
+           (fol.impH  (fol.equal L (fol.var L 0) (fol.var L 1))
               (fol.equal L (fol.var L 1) (fol.var L 0)))) with C;
         [ idtac | reflexivity ].
       generalize C; intros C0.
@@ -2165,8 +2164,8 @@ Repeat First [Rewrite cPairProjections1|Rewrite cPairProjections2].
       unfold checkPrfEQ3 in |- *.
       replace
         (codeFormula L codeF codeR
-           (fol.impH L (fol.equal L (fol.var L 0) (fol.var L 1))
-              (fol.impH L (fol.equal L (fol.var L 1) (fol.var L 2))
+           (fol.impH (fol.equal L (fol.var L 0) (fol.var L 1))
+              (fol.impH (fol.equal L (fol.var L 1) (fol.var L 2))
                  (fol.equal L (fol.var L 0) (fol.var L 2))))) 
         with C; [ idtac | reflexivity ].
       generalize C; intros.
@@ -2614,7 +2613,7 @@ Proof.
                       (cPair (codeFormula L codeF codeR x2) 
                          (codeFormula L codeF codeR x)))
                    with (codeFormula L codeF codeR x1).
-                 { rewrite H14; fold impH; rewrite H15; rewrite H13.
+                 { rewrite H14;  rewrite H15; rewrite H13.
                    rewrite cPairProjections; reflexivity.
                  } 
                } 
@@ -3260,13 +3259,13 @@ Proof.
                       induction
                         (eq_nat_dec
                            (codeFormula L codeF codeR
-                              (fol.impH L (fol.equal L (fol.var L 0) 
+                              (fol.impH (fol.equal L (fol.var L 0) 
                                              (fol.var L 1))
                                  (fol.equal L (fol.var L 1) (fol.var L 0))))
                            (codeFormula L codeF codeR x)).
                       rewrite H3.
                       replace x with
-                        (fol.impH L (fol.equal L (fol.var L 0) (fol.var L 1))
+                        (fol.impH (fol.equal L (fol.var L 0) (fol.var L 1))
                            (fol.equal L (fol.var L 1) (fol.var L 0))).
                       exists (EQ2 L).
                       simpl in |- *.
@@ -3287,7 +3286,7 @@ Proof.
                       rewrite
                         (nat_eqb_false
                            (codeFormula L codeF codeR
-                              (fol.impH L (fol.equal L (fol.var L 0) (fol.var L 1))
+                              (fol.impH (fol.equal L (fol.var L 0) (fol.var L 1))
                                  (fol.equal L (fol.var L 1) (fol.var L 0))))).
                       
                       rewrite Nat.mul_comm.
@@ -3313,14 +3312,14 @@ Simpl in H0.
                       induction
                         (eq_nat_dec
                            (codeFormula L codeF codeR
-                              (fol.impH L (fol.equal L (fol.var L 0) (fol.var L 1))
-                                 (fol.impH L (fol.equal L (fol.var L 1) (fol.var L 2))
+                              (fol.impH (fol.equal L (fol.var L 0) (fol.var L 1))
+                                 (fol.impH (fol.equal L (fol.var L 1) (fol.var L 2))
                                     (fol.equal L (fol.var L 0) (fol.var L 2)))))
                            (codeFormula L codeF codeR x)).
                       rewrite H3.
                       replace x with
-                        (fol.impH L (fol.equal L (fol.var L 0) (fol.var L 1))
-                           (fol.impH L (fol.equal L (fol.var L 1) (fol.var L 2))
+                        (fol.impH (fol.equal L (fol.var L 0) (fol.var L 1))
+                           (fol.impH (fol.equal L (fol.var L 1) (fol.var L 2))
                               (fol.equal L (fol.var L 0) (fol.var L 2)))).
                       exists (EQ3 L).
                       simpl in |- *.
@@ -3342,9 +3341,9 @@ Simpl in H0.
                       rewrite
                         (nat_eqb_false
                            (codeFormula L codeF codeR
-                              (fol.impH L (fol.equal L (fol.var L 0) 
+                              (fol.impH (fol.equal L (fol.var L 0) 
                                              (fol.var L 1))
-                                 (fol.impH L (fol.equal L (fol.var L 1) 
+                                 (fol.impH (fol.equal L (fol.var L 1) 
                                                 (fol.var L 2))
                                     (fol.equal L (fol.var L 0) 
                                        (fol.var L 2))))))
